IMP-_To_SAS+/IMP-_To_IMP--/IMP_Minus_To_IMP_Minus_Minus_State_Translations.thy
@@ -61,7 +61,7 @@ proof
         takeWhile_dropWhile_id tl_append2)
 qed auto
 
-lemma var_bit_to_var_eq_iff: "var_bit_to_var (a, b) = var_bit_to_var (c, d) \<longleftrightarrow> (a = c \<and> b = d)" 
+lemma var_bit_to_var_eq_iff[simp]: "var_bit_to_var (a, b) = var_bit_to_var (c, d) \<longleftrightarrow> (a = c \<and> b = d)" 
   apply(auto simp: var_bit_to_var_def)
    apply (metis dropWhile_n_hashes list.inject)
   by (metis length_takeWhile_n_hashes)
@@ -124,57 +124,5 @@ lemma IMP_Minus_State_To_IMP_Minus_Minus_of_non_zero_indicator_of_carry[simp]:
 lemma is_non_zero_indicator_iff: "take 2 x = ''?$''
   \<longleftrightarrow> x = ''?$'' @ drop 2 x" 
   by (metis append_same_eq append_take_drop_id)
-
-fun atomExp_to_constant:: "AExp.atomExp \<Rightarrow> nat" where
-"atomExp_to_constant (AExp.V var) = 0" |
-"atomExp_to_constant (AExp.N val) = val"
-
-fun aexp_max_constant:: "AExp.aexp \<Rightarrow> nat" where
-"aexp_max_constant (AExp.A a) = atomExp_to_constant a" |
-"aexp_max_constant (AExp.Plus a b) = max (atomExp_to_constant a) (atomExp_to_constant b)" |
-"aexp_max_constant (AExp.Sub a b) = max (atomExp_to_constant a) (atomExp_to_constant b)"
-
-fun max_constant :: "Com.com \<Rightarrow> nat" where
-"max_constant (Com.SKIP) = 0" |
-"max_constant (Com.Assign vname aexp) = aexp_max_constant aexp" |
-"max_constant (Com.Seq c1  c2) = max (max_constant c1) (max_constant c2)" |         
-"max_constant (Com.If  _ c1 c2) = max (max_constant c1) (max_constant c2)"  |   
-"max_constant (Com.While _ c) = max_constant c"
-
-lemma Max_range_le_then_element_le: "finite (range s) \<Longrightarrow> 2 * Max (range s) < (x :: nat) \<Longrightarrow> 2 * (s y) < x" 
-proof -
-  assume "2 * Max (range s) < (x :: nat)"
-  moreover have "s y \<in> range s" by simp
-  moreover assume "finite (range s)" 
-  moreover hence "s y \<le> Max (range s)" by simp
-  ultimately show ?thesis by linarith
-qed
-
-lemma aval_le_when: 
-  assumes "finite (range s)" "2 * max (Max (range s)) (aexp_max_constant a) < x" 
-  shows "AExp.aval a s < x"
-using assms proof(cases a)
-  case (A x1)
-  thus ?thesis using assms
-  proof(cases x1)
-    case (V x2)
-    thus ?thesis using assms A Max_range_le_then_element_le[where ?s=s and ?x = x and ?y=x2] by simp
-  qed simp
-next
-  case (Plus x21 x22)
-  hence "2 * max (AExp.atomVal x21 s) (AExp.atomVal x22 s) < x" 
-    apply(cases x21; cases x22)
-    using assms 
-    by (auto simp add: Max_range_le_then_element_le nat_mult_max_right)
-  thus ?thesis using Plus by auto
-next
-  case (Sub x31 x32)
-  then show ?thesis 
-    apply(cases x31 ; cases x32)
-    using assms apply(auto simp add: Max_range_le_then_element_le nat_mult_max_right)
-    using Max_range_le_then_element_le 
-    by (metis gr_implies_not0 lessI less_imp_diff_less less_imp_le_nat less_le_trans 
-        linorder_neqE_nat n_less_m_mult_n numeral_2_eq_2)+
-qed
 
 end
